Break up polycompilers into 3 files

src/Pyrosome/Lang/PolyCompilers.v
@@ -17,767 +17,15 @@ From Pyrosome.Lang Require Import PolySubst
   SimpleVSubst SimpleVCPS SimpleEvalCtx Let
   SimpleEvalCtxCPS SimpleUnit NatHeap SimpleVCPSHeap
   SimpleVFixCPS SimpleVFixCC SimpleVCC SimpleVSTLC
-  SimpleVCCHeap SimpleVFix CombinedThm.
+  SimpleVCCHeap SimpleVFix CombinedThm PolyCompilerLangs PolyCompilersCPS.
+From Pyrosome.Tools Require Import InjRuleGen.
+From Pyrosome.Tools Require Import UnElab.
+From Pyrosome.Compilers Require Import CompilerTransitivity.
 Import Core.Notations.
 Import CompilerDefs.Notations.
 
 From Stdlib Require derive.Derive.
-
-Definition stlc_parameterized :=
-    let ps := (elab_param "D" (stlc ++ exp_ret ++ exp_subst_base
-                                 ++ value_subst)
-               [("sub", Some 2);
-                ("ty", Some 0);
-                ("env", Some 0);
-                ("val",Some 2);
-                ("exp",Some 2)]) in
-  parameterize_lang "D" {{s #"ty_env"}}
-    ps stlc.
-
-Local Definition evp' := 
-    let ps := (elab_param "D" (stlc ++exp_ret ++ exp_subst_base
-                                 ++ value_subst)
-               [("sub", Some 2);
-                ("ty", Some 0);
-                ("env", Some 0);
-                ("val",Some 2);
-                ("exp",Some 2)]) in
-  parameterize_lang "D" {{s #"ty_env"}}
-    ps (exp_ret ++ exp_subst_base ++ value_subst).
-
-Lemma stlc_parameterized_wf
-  : wf_lang_ext ((exp_parameterized++val_parameterized)
-                       ++ty_env_lang)
-      stlc_parameterized.
-Proof.
-  change (exp_parameterized++val_parameterized) with evp'.
-  (*TODO: phrase exp_and_val_parameterized as parameterized in definition*)
-  (*TODO: need to strengthen parameterization pl w/ add'l language?
-    Currently cheating.
-   *)
-  eapply parameterize_lang_preserving_ext;
-    try typeclasses eauto;
-    [repeat t';  constructor (*TODO: include in t'*)
-    | now prove_by_lang_db..
-    | vm_compute; exact I].
-Qed.
-#[local] Definition stlc_parameterized_entry :=
-  lang_entry stlc_parameterized_wf.
-#[export] Hint Resolve stlc_parameterized_entry : wf_lang_db.
-
-Definition src_parameterized :=
-    let ps := (elab_param "D" (let_lang ++ src_ext ++ exp_ret ++ exp_subst_base
-                                 ++ value_subst)
-               [("sub", Some 2);
-                ("ty", Some 0);
-                ("env", Some 0);
-                ("val",Some 2);
-                ("exp",Some 2)]) in
-  parameterize_lang "D" {{s #"ty_env"}}
-    ps (let_lang ++ src_ext).
-
-Local Definition evp'' := 
-    let ps := (elab_param "D" (let_lang ++ src_ext ++exp_ret ++ exp_subst_base
-                                 ++ value_subst)
-               [("sub", Some 2);
-                ("ty", Some 0);
-                ("env", Some 0);
-                ("val",Some 2);
-                ("exp",Some 2)]) in
-  parameterize_lang "D" {{s #"ty_env"}}
-    ps (exp_subst ++ value_subst).
-
-(*TODO: move to Core.v*)
-Lemma wf_lang_concat' (l_pre l1 l2 : lang)
-  : wf_lang_ext l_pre l1 ->
-    wf_lang_ext (l1++l_pre) l2 ->
-    wf_lang_ext l_pre (l2 ++ l1).
-Proof.
-  induction 2; basic_goal_prep; basic_core_firstorder_crush.
-  rewrite <- app_assoc; eauto.
-Qed.
-
-Lemma src_parameterized_wf
-  : wf_lang_ext ((exp_parameterized++val_parameterized)
-                       ++ty_env_lang)
-      src_parameterized.
-Proof.
-  change (exp_parameterized++val_parameterized) with evp''.
-  eapply parameterize_lang_preserving_ext;
-    try typeclasses eauto;
-    [repeat t';  constructor (*TODO: include in t'*)
-    | try now prove_by_lang_db..
-    | vm_compute; exact I].
-Qed.
-#[local] Definition src_parameterized_entry :=
-  lang_entry src_parameterized_wf.
-#[export] Hint Resolve src_parameterized_entry : wf_lang_db.
-
-(*TODO: move to a better place*)
-Definition hide_ccase_implicits {V} `{Eqb V} `{WithDefault V}
-  (tgt : Rule.lang V) (cc: compiler_case V) :=
-  match cc with
-  | sort_case args t =>
-      sort_case args (Rule.hide_sort_implicits tgt t)
-  | term_case args e =>
-      term_case args (Rule.hide_term_implicits tgt e)
-  end.
-
-Definition hide_compiler {V} `{Eqb V} `{WithDefault V} (l : Rule.lang V)
-  : CompilerDefs.compiler V -> _:=
-  NamedList.named_map (hide_ccase_implicits l).
-
-
-Definition cps_full := (let_cps++fix_cps++ cps ++ heap_ctx_cps ++ Ectx_cps++ heap_cps++heap_id++cps_subst++[]).
-
-Definition ir_parameterized :=
-  let ps := (elab_param "D" (ir_ext ++ block_subst
-                                 ++ value_subst)
-               [("sub", Some 2);
-                ("ty", Some 0);
-                ("env", Some 0);
-                ("val",Some 2);
-                ("blk",Some 1)]) in
-  parameterize_lang "D" {{s #"ty_env"}}
-    ps ir_ext.
-
-Local Definition bvp' :=
-  let ps := (elab_param "D" (ir_ext
-                               ++ block_subst
-                                 ++ value_subst)
-               [("sub", Some 2);
-                ("ty", Some 0);
-                ("env", Some 0);
-                ("val",Some 2);
-                ("blk",Some 1)]) in
-  parameterize_lang "D" {{s #"ty_env"}}
-    ps (block_subst ++ value_subst).
-
-Lemma ir_parameterized_wf
-  : wf_lang_ext ((block_parameterized++
-                       val_parameterized)
-                       ++ty_env_lang)
-      ir_parameterized.
-Proof.
-  change (block_parameterized++val_parameterized) with bvp'.
-  eapply parameterize_lang_preserving_ext;
-    try typeclasses eauto;
-    [repeat t';  constructor (*TODO: include in t'*)
-    | try now  prove_by_lang_db..
-    | vm_compute; exact I].
-Qed.
-#[local] Definition ir_parameterized_entry :=
-  lang_entry ir_parameterized_wf.
-#[export] Hint Resolve ir_parameterized_entry : wf_lang_db.
-
-Definition cps_parameterized :=
-    (*TODO: elab_param seems to do the right thing, why is
-      parameterize_compiler doing the wrong thing with it?
-     *)
-    let ps := (elab_param "D" (let_lang ++ src_ext ++ exp_ret ++ exp_subst_base
-                                 ++ value_subst)
-               [("sub", Some 2);
-                ("ty", Some 0);
-                ("env", Some 0);
-                ("val",Some 2);
-                ("exp",Some 2)]) in
-    let pir :=  (elab_param "D" (ir_ext ++ block_subst
-                                 ++ value_subst)
-               [("sub", Some 2);
-                ("ty", Some 0);
-                ("env", Some 0);
-                ("val",Some 2);
-                ("blk",Some 1)]) in
-    parameterize_compiler "D"
-      (*firstn 44 skips the rule for ty. TODO: still necessary?*)
-      pir ps cps_full.
-
-Definition ty_env_cmp := id_compiler ty_env_lang.
-
-(*TODO: prove the more general version*)
-From Pyrosome Require Import Theory.Core Compilers.Compilers Elab.ElabCompilers.
-Lemma ty_subst_id_compiler_correct
-  : (preserving_compiler_ext
-       (tgt_Model:=core_model ty_env_lang)
-       []
-       ty_env_cmp
-       ty_env_lang).
-Proof.
-  apply id_compiler_preserving; try typeclasses eauto.
-  prove_by_lang_db.
-Qed.
-#[local] Definition ty_subst_id_entry :=
-  cmp_entry ty_subst_id_compiler_correct.
-#[export] Hint Resolve ty_subst_id_entry : preserving_db.     
-
-Lemma cps_parameterized_correct
-  : preserving_compiler_ext
-      (tgt_Model:=core_model ((ir_parameterized
-                                ++ (block_parameterized++
-                                      val_parameterized))
-                                ++ty_env_lang))
-      ty_env_cmp
-      cps_parameterized
-      (src_parameterized
-         ++ (exp_parameterized++
-               val_parameterized)).
-Proof.
-  change (exp_parameterized++val_parameterized) with evp''.
-  unfold ty_env_cmp, cps_parameterized,
-    src_parameterized, evp''.
-  unfold parameterize_lang.
-  rewrite <- map_app.
-  match goal with
-  | |- context[core_model ?l] =>
-      let y := type of l in
-      let x := open_constr:(_:y) in
-      replace (core_model l) with (core_model x)
-  end.
-  1:eapply parameterize_compiler_preserving.
-  all: try typeclasses eauto.
-  1,2:repeat t'; try constructor.
-  1: eapply use_compute_all_fresh; vm_compute; exact I.
-  2:rewrite <- app_assoc; eapply full_cps_compiler_preserving.
-  1:prove_by_lang_db.
-  1:prove_by_lang_db.
-  2: reflexivity.
-  1: vm_cast_no_check I.
-Qed.
-#[local] Definition cps_parameterized_entry :=
-  cmp_entry cps_parameterized_correct.
-#[export] Hint Resolve cps_parameterized_entry : preserving_db.
-
 Local Open Scope lang_scope.
-Definition exists_def : lang _ :=
-  {[l (*l/subst TODO: psubst*)
-  [:| "D" : #"ty_env", "A" : #"ty" (#"ty_ext" "D")
-      -----------------------------------------------
-      #"Exists" "A" : #"ty" "D"
-  ];
-    (*TODO:autogenerate*)
-  [:= "D" : #"ty_env",
-      "A" : #"ty" (#"ty_ext" "D"),
-      "D'" : #"ty_env",
-      "d" : #"ty_sub" "D'" "D"
-      ----------------------------------------------- ("ty_subst Exists")
-      #"ty_subst" "d" (#"Exists" "A")
-      = #"Exists" (#"ty_subst" (#"ty_snoc" (#"ty_cmp" #"ty_wkn" "d") #"ty_hd") "A")
-      : #"ty" "D'"
-   ];
-    [:| "D" : #"ty_env",
-       "G" : #"env" "D",
-       "A" :  #"ty" "D",
-       "B" :  #"ty" (#"ty_ext" "D"),
-       "v" : #"val" "D" "G" (#"ty_subst" (#"ty_snoc" #"ty_id" "A") "B")
-       -----------------------------------------------
-       #"pack_val" "A" "v" : #"val" "D" "G" (#"Exists" "B")
-  ];
-    [:| "D" : #"ty_env",
-       "G" : #"env" "D",
-       "A" :  #"ty" "D",
-       "B" :  #"ty" (#"ty_ext" "D"),
-       "e" : #"exp" "D" "G" (#"ty_subst" (#"ty_snoc" #"ty_id" "A") "B")
-       -----------------------------------------------
-       #"pack" "A" "e" : #"exp" "D" "G" (#"Exists" "B")
-  ];
-  [:| "D" : #"ty_env",
-      "G" : #"env" "D",
-      "B" : #"ty" (#"ty_ext" "D"),
-      "e" : #"exp" "D" "G" (#"Exists" "B"),
-      "C" : #"ty" "D",
-      "e'" : #"exp" (#"ty_ext" "D") (#"ext" (#"env_ty_subst" #"ty_wkn" "G") "B")
-               (#"ty_subst" #"ty_wkn" "C")
-       -----------------------------------------------
-       #"unpack" "e" "e'" : #"exp" "D" "G" "C"
-  ];
-  [:=  "D" : #"ty_env",
-       "G" : #"env" "D",
-       "A" :  #"ty" "D",
-       "B" :  #"ty" (#"ty_ext" "D"),
-       "v" : #"val" "D" "G" (#"ty_subst" (#"ty_snoc" #"ty_id" "A") "B"),
-      "C" : #"ty" "D",
-      "e'" : #"exp" (#"ty_ext" "D") (#"ext" (#"env_ty_subst" #"ty_wkn" "G") "B")
-               (#"ty_subst" #"ty_wkn" "C")
-      ----------------------------------------------- ("unpack-beta")
-      #"unpack" (#"ret" (#"pack_val" "A" "v")) "e'"
-      = #"exp_subst" (#"snoc" #"id" "v") (#"exp_ty_subst" (#"ty_snoc" #"ty_id" "A") "e'")
-      : #"exp" "D" "G" "C"
-  ]
-  ]}.
-
-#[local] Definition Exists_inst_for_db := inst_for_db "Exists".
-#[export] Hint Resolve Exists_inst_for_db : injective_con.
-
-(*TODO: move to top of file*)
-From Pyrosome.Tools Require Import InjRuleGen.
-
-Definition exists_lang :=
-  Eval vm_compute in
-    (infer_lang_ext_simple_incr 10 100
-       (exp_param_substs
-          ++ exp_ty_subst
-          ++ val_param_substs
-          ++ val_ty_subst
-          ++env_ty_subst
-          ++ty_subst_lang
-          ++exp_parameterized++val_parameterized
-          ++ty_env_lang) exists_def).
-
-
-Lemma exists_lang_wf : wf_lang_ext (exp_param_substs
-                             ++ exp_ty_subst
-                             ++ val_param_substs
-                             ++ val_ty_subst
-                             ++env_ty_subst
-                             ++ty_subst_lang
-                             ++exp_parameterized++val_parameterized
-                             ++ty_env_lang)
-                               exists_lang.
-Proof. compute_wf_lang. Qed.
-#[local] Definition exists_lang_entry :=
-  lang_entry exists_lang_wf.
-#[export] Hint Resolve exists_lang_entry : wf_lang_db.
-
-Definition exists_block_def : lang _ :=
-  {[l (*l/subst TODO: psubst*)
-  [:| "D" : #"ty_env", "A" : #"ty" (#"ty_ext" "D")
-      -----------------------------------------------
-      #"Exists" "A" : #"ty" "D"
-  ];
-    [:= "D" : #"ty_env",
-              "A" : #"ty" (#"ty_ext" "D"),
-              "D'" : #"ty_env",
-              "d" : #"ty_sub" "D'" "D"
-              ----------------------------------------------- ("ty_subst Exists")
-              #"ty_subst" "d" (#"Exists" "A")
-               = #"Exists" (#"ty_subst" (#"ty_snoc" (#"ty_cmp" #"ty_wkn" "d") #"ty_hd") "A")
-               : #"ty" "D'"
-          ];
-    [:| "D" : #"ty_env",
-       "G" : #"env" "D",
-       "A" :  #"ty" "D",
-       "B" :  #"ty" (#"ty_ext" "D"),
-       "v" : #"val" "D" "G" (#"ty_subst" (#"ty_snoc" #"ty_id" "A") "B")
-       -----------------------------------------------
-       #"pack" "A" "v" : #"val" "D" "G" (#"Exists" "B")
-  ];
-  [:| "D" : #"ty_env",
-      "G" : #"env" "D",
-      "B" : #"ty" (#"ty_ext" "D"),
-      "v" : #"val" "D" "G" (#"Exists" "B"),
-      "e" : #"blk" (#"ty_ext" "D") (#"ext" (#"env_ty_subst" #"ty_wkn" "G") "B")
-       -----------------------------------------------
-       #"unpack" "v" "e" : #"blk" "D" "G"
-  ];
-  [:=  "D" : #"ty_env",
-       "G" : #"env" "D",
-       "A" :  #"ty" "D",
-       "B" :  #"ty" (#"ty_ext" "D"),
-       "v" : #"val" "D" "G" (#"ty_subst" (#"ty_snoc" #"ty_id" "A") "B"),
-      "e" : #"blk" (#"ty_ext" "D") (#"ext" (#"env_ty_subst" #"ty_wkn" "G") "B")
-      ----------------------------------------------- ("unpack-beta")
-      #"unpack" (#"pack" "A" "v") "e"
-      = #"blk_subst" (#"snoc" #"id" "v") (#"blk_ty_subst" (#"ty_snoc" #"ty_id" "A")"e")
-      : #"blk" "D" "G"
-  ];
-  [:= "D" : #"ty_env",
-      "G" : #"env" "D",
-      "B" : #"ty" (#"ty_ext" "D"),
-      "v" : #"val" "D" "G" (#"Exists" "B"),
-      "e" : #"blk" "D" (#"ext" "G" (#"Exists" "B"))
-       ----------------------------------------------- ("unpack-eta")
-       #"unpack" "v" (#"blk_subst" (#"snoc" #"wkn" (#"pack" #"ty_hd" #"hd"))
-                        (#"blk_ty_subst" #"ty_wkn" "e"))
-       = #"blk_subst" (#"snoc" #"id" "v") "e"
-       : #"blk" "D" "G"
-  ];
-   [:= "D" : #"ty_env",
-       "G" : #"env" "D",
-       "A" :  #"ty" "D",
-       "B" :  #"ty" (#"ty_ext" "D"),
-       "v" : #"val" "D" "G" (#"ty_subst" (#"ty_snoc" #"ty_id" "A") "B"),
-      "G'" : #"env" "D",
-      "g" : #"sub" "D" "G'" "G"
-       ----------------------------------------------- ("blk_subst pack")
-       #"val_subst" "g" (#"pack" "A" "v")
-       = #"pack" "A" (#"val_subst" "g" "v")
-       : #"val" "D" "G'" (#"Exists" "B")
-  ];
-  [:= "D" : #"ty_env",
-      "G" : #"env" "D",
-      "B" : #"ty" (#"ty_ext" "D"),
-      "v" : #"val" "D" "G" (#"Exists" "B"),
-      "e" : #"blk" (#"ty_ext" "D") (#"ext" (#"env_ty_subst" #"ty_wkn" "G") "B"),
-      "G'" : #"env" "D",
-      "g" : #"sub" "D" "G'" "G"
-       ----------------------------------------------- ("blk_subst unpack")
-       #"blk_subst" "g" (#"unpack" "v" "e")
-       = #"unpack" (#"val_subst" "g" "v")
-           (#"blk_subst" { under {{e #"sub_ty_subst" #"ty_wkn" "g" }} } "e")
-       : #"blk" "D" "G'"
-  ]
-  ]}.
-
-
-Definition exists_block_lang' :=
-  Eval vm_compute in
-    (infer_lang_ext_simple_incr 10 100
-       (block_param_substs
-          ++val_param_substs
-          ++ block_ty_subst
-          ++env_ty_subst
-          ++ty_subst_lang
-          ++block_parameterized++val_parameterized
-          ++ty_env_lang)
-       exists_block_def).
-
-(*TODO: too slow. Why? should replace the derive below.
-Lemma exists_block_lang_wf
-  : wf_lang_ext (block_param_substs
-                   ++val_param_substs
-                   ++ block_ty_subst
-                   ++env_ty_subst
-                   ++ty_subst_lang
-                   ++block_parameterized++val_parameterized
-                   ++ty_env_lang)
-      exists_block_lang.
-Proof. compute_wf_lang. Qed.
-*)
-
-Derive exists_block_lang
-  in (elab_lang_ext (block_param_substs
-                             ++val_param_substs
-                             ++ block_ty_subst
-                             ++env_ty_subst
-                             ++ty_subst_lang
-                             ++block_parameterized++val_parameterized
-                             ++ty_env_lang)
-              exists_block_def exists_block_lang)
-       as exists_block_lang_wf.
-Proof. auto_elab. Qed.
-#[local] Definition exists_block_lang_entry :=
-  lang_entry (elab_lang_implies_wf exists_block_lang_wf).
-#[export] Hint Resolve exists_block_lang_entry : wf_lang_db.
-
-Definition exp_ty_subst_cps_def : compiler string :=
-  match # from (exp_param_substs ++ exp_ty_subst) with
-  | {{e #"exp_ty_subst" "D" "D'" "g" "G" "A" "e"}} =>
-      {{e #"blk_ty_subst" "g" "e"}}
-  end.
-
-From Pyrosome.Tools Require Import UnElab.
-
-Definition ir_param_substs_def :=
-  Eval compute in
-    let deps := (block_param_substs
-                                 ++ val_param_substs
-                                 ++ block_ty_subst
-                                 ++ env_ty_subst
-                                 ++ ty_subst_lang
-                                 ++ block_parameterized
-                                 ++ val_parameterized
-                                 ++ ty_env_lang) in
-    eqn_rules type_subst_mode deps
-    (hide_lang_implicits (ir_parameterized++deps) ir_parameterized).
-
-(*TODO: this takes too long. Why?
-Definition ir_param_substs :=
-  Eval vm_compute in
-    (infer_lang_ext_simple_incr 10 100
-       (block_param_substs
-          ++ val_param_substs
-          ++ block_ty_subst
-          ++ env_ty_subst
-          ++ ty_subst_lang
-          ++ block_parameterized
-          ++ val_parameterized
-          ++ ty_env_lang)
-       ir_param_substs_def).
-*)
-
-Derive ir_param_substs
-  in (elab_lang_ext (ir_parameterized
-                             ++block_param_substs
-                             ++val_param_substs
-                             ++block_ty_subst
-                             ++env_ty_subst
-                             ++block_parameterized
-                             ++ty_subst_lang
-                             ++val_parameterized
-                             ++ty_env_lang)
-              ir_param_substs_def
-              ir_param_substs)
-  as ir_param_substs_wf.
-Proof. auto_elab. Qed.
-#[local] Definition ir_param_substs_entry :=
-  lang_entry (elab_lang_implies_wf ir_param_substs_wf).
-#[export] Hint Resolve ir_param_substs_entry : wf_lang_db.
-
-Definition exp_ty_subst_cps' :=
-  Eval vm_compute in
-    (infer_compiler_simple_autoinj 7
-       (ir_param_substs
-                 ++ ir_parameterized (*TODO: only include conts*)
-                 ++ block_param_substs
-                 ++ val_param_substs
-                 ++ block_ty_subst
-                 ++env_ty_subst
-                 ++ty_subst_lang
-                 ++block_parameterized++val_parameterized
-                 ++ty_env_lang)
-       (id_compiler (val_param_substs
-                             ++ val_ty_subst
-                              ++env_ty_subst
-                              ++ty_subst_lang)
-                 ++ cps_parameterized++ty_env_cmp)
-       exp_ty_subst_cps_def
-       (exp_param_substs ++ exp_ty_subst)).
-
-(* TODO: Qed/e-graph fails. Why?
-Lemma cps_preserving
-  : preserving_compiler_ext
-      (id_compiler (val_param_substs
-                      ++ val_ty_subst
-                      ++env_ty_subst
-                      ++ty_subst_lang)
-         ++ cps_parameterized++ty_env_cmp)
-      (tgt_Model:= core_model
-                     (ir_param_substs
-                        ++ ir_parameterized (*TODO: only include conts*)
-                        ++ block_param_substs
-                        ++ val_param_substs
-                        ++ block_ty_subst
-                        ++env_ty_subst
-                        ++ty_subst_lang
-                        ++block_parameterized++val_parameterized
-                        ++ty_env_lang))
-      exp_ty_subst_cps
-      (exp_param_substs ++ exp_ty_subst).
-Proof.
-  compute_preserving_compiler
-    ((val_param_substs
-        ++ val_ty_subst
-        ++env_ty_subst
-        ++ty_subst_lang)
-       ++(src_parameterized ++ exp_parameterized ++ val_parameterized)
-       ++ty_env_lang).
-Qed.
-*)
-
-Derive exp_ty_subst_cps
-  in (elab_preserving_compiler
-              (id_compiler (val_param_substs
-                             ++ val_ty_subst
-                              ++env_ty_subst
-                              ++ty_subst_lang)
-                 ++ cps_parameterized++ty_env_cmp)
-              (ir_param_substs
-                 ++ ir_parameterized (*TODO: only include conts*)
-                 ++ block_param_substs
-                 ++ val_param_substs
-                 ++ block_ty_subst
-                 ++env_ty_subst
-                 ++ty_subst_lang
-                 ++block_parameterized++val_parameterized
-                 ++ty_env_lang)
-              exp_ty_subst_cps_def
-              exp_ty_subst_cps
-              (exp_param_substs ++ exp_ty_subst))
-  as exp_ty_subst_cps_preserving.
-Proof. auto_elab_compiler. Qed.
-#[local] Definition exp_ty_subst_cps_entry :=
-  cmp_entry (elab_compiler_implies_preserving exp_ty_subst_cps_preserving).
-#[export] Hint Resolve exp_ty_subst_cps_entry : preserving_db.
-
-Definition poly_cps_def : compiler string :=
-  match # from poly with
-  | {{e #"All" "D" "A"}} =>
-    {{e #"neg" (#"Exists" (#"neg" "A")) }}
-  | {{e #"Lam" "D" "G" "A" "e"}} =>
-      {{e #"cont" (#"Exists" (#"neg" "A"))
-          (#"unpack" #"hd" (#"blk_subst" (#"snoc" (#"cmp" #"wkn" #"wkn") #"hd") "e")) }}
-  | {{e #"@" "D" "G" "A" "e" "B"}} =>      
-    bind_k 1 (var "e") {{e #"neg" (#"Exists" (#"neg" "A")) }}
-    {{e #"jmp" {ovar 0} (#"pack" "B" {ovar 1}) }}
-  end.
-
-(*TODO: move somewhere*)
-Definition count_constr_implicits (l:lang string) n :=
-  match named_list_lookup_err l n with
-  | Some (sort_rule c args)
-  | Some (term_rule c args _) => length c - length args
-  | _ => 0
-  end.
-
-Fixpoint count_implicits l e :=
-  match e with
-  | var _ => 0
-  | con n s =>
-      fold_left Nat.add (map (count_implicits l) s) (count_constr_implicits l n)
-  end.
-Import Monad.
-Import StateMonad.
-
-Local Notation ctx := (ctx string).
-Local Notation term := (term string).
-Local Notation lang := (lang string).
-Definition ask_evar : state (list term) term :=
-  fun l => (hd default l, tl l).
-
-(*TODO: no fuel*)
-Section __.
-  Context (insert_implicits : term -> state (list term) term).
-
-  Fixpoint insert_implicits_args (fuel : nat)
-    (c:ctx) args s {struct fuel} : state (list term) (list term) :=
-    match fuel with
-    | S fuel =>
-        match c, args, s with
-        | [], [], [] => Mret []
-        | (x,_)::c', [], [] =>
-            @! let x_evar <- ask_evar in
-              let s' <- insert_implicits_args fuel c' [] [] in
-              ret x_evar::s'
-        | (x,_)::c', y::args', e::s' =>
-            if eqb x y then
-              @! let s'' <- insert_implicits_args fuel c' args' s' in
-                let e' <- insert_implicits e in
-                ret e':: s''
-            else
-              @! let x_evar <- ask_evar in
-                let s'' <- insert_implicits_args fuel c' args s in
-                ret x_evar::s''
-        | _, _, _ => Mret default
-        end
-    | O => Mret default
-    end.
-End __.
-(*really want a reader monad, but I don't have that *)
-Fixpoint insert_implicits fuel l e {struct fuel} : state (list term) term :=
-  match fuel with
-  | S fuel =>
-      match e with
-      | var x => Mret (var x)
-      | con n s =>
-          match  (named_list_lookup_err l n) with
-          | Some (term_rule c args _) =>
-              @! let s' <- insert_implicits_args (insert_implicits fuel l) fuel c args s in
-                ret con n s'
-          | _ => Mret default
-          end
-      end
-  | O => Mret default
-  end.
-
-Ltac mk_evar_list c :=
-  lazymatch c with
-  | S ?c' =>
-      let x := open_constr:(_:term) in
-      let l' := mk_evar_list c' in
-      constr:(x::l')
-  | O => constr:([])
-  end.
-
-Ltac insert_implicits l e :=
-  let c := eval compute in (count_implicits l e) in
-    let evar_list := mk_evar_list c in
-    let e' := eval compute in (snd (insert_implicits 100 l e evar_list)) in
-      idtac e'.
-
-
-Ltac intermediate_term e :=      
-  match goal with
-    |- eq_term ?l' ?c ?t ?e1 ?e2 =>
-      let e' := open_constr:(_:term) in
-      assert (elab_term l' c e e' t) as H';
-      [| eapply eq_term_trans with (e12:=e');
-         clear H']
-  end.
-
-(* Temporary until I restore the proof*)
-Axiom (TODO : forall {A}, A).
-Derive poly_cps
-  in (elab_preserving_compiler
-              (exp_ty_subst_cps
-                 ++ id_compiler (val_param_substs
-                                   ++ val_ty_subst
-                                   ++env_ty_subst
-                                   ++ty_subst_lang)
-                 ++ cps_parameterized++ty_env_cmp)
-              (exists_block_lang
-                 ++ ir_param_substs
-                 ++ ir_parameterized (*TODO: only include conts*)
-                 ++ block_param_substs
-                 ++ val_param_substs
-                 ++ block_ty_subst
-                 ++env_ty_subst
-                 ++ty_subst_lang
-                 ++block_parameterized++val_parameterized
-                 ++ty_env_lang)
-              poly_cps_def
-              poly_cps
-              poly)
-  as poly_cps_preserving.
-Proof.
-  auto_elab_compiler.
-  {  apply TODO (*Automation.by_reduction; t'.*). }
-  (*Automation.auto_elab_compiler.
-12:57-1:46+; too long
-   *)
-Qed.
-#[local] Definition poly_cps_entry :=
-  cmp_entry (elab_compiler_implies_preserving poly_cps_preserving).
-#[export] Hint Resolve poly_cps_entry : preserving_db.
-
-Local Definition unpack_swap :=
-  {{e #"snoc" (#"snoc" (#"cmp" (#"cmp" #"wkn" #"wkn") #"wkn") #"hd") {ovar 2} }}.
-
-Definition exists_cps_def : compiler string :=
-  match # from exists_lang with
-  | {{e #"Exists" "D" "A"}} =>
-      {{e #"Exists" "A" }}
-  | {{e #"pack_val" "D" "G" "A" "B" "v"}} =>
-      {{e #"pack" "A" "v" }}
-  | {{e #"pack" "D" "G" "A" "B" "e"}} =>
-      bind_k 1 (var "e") {{e #"ty_subst" (#"ty_snoc" #"ty_id" "A") "B" }}
-        {{e #"jmp" {ovar 1} (#"pack" "A" #"hd") }}
-  | {{e #"unpack" "D" "G" "B" "e" "C" "e'" }} =>
-    bind_k 1 (var "e") {{e #"Exists" "B" }}
-      {{e #"unpack" #"hd" (#"blk_subst" {unpack_swap} "e'")  }}
-  end.
-
-Derive exists_cps
-  in (elab_preserving_compiler
-              (exp_ty_subst_cps
-                 ++ id_compiler (val_param_substs
-                                   ++ val_ty_subst
-                                   ++env_ty_subst
-                                   ++ty_subst_lang)
-                 ++ cps_parameterized++ty_env_cmp)
-              (exists_block_lang
-                 ++ ir_param_substs
-                 ++ ir_parameterized (*TODO: only include conts*)
-                 ++ block_param_substs
-                 ++ val_param_substs
-                 ++ block_ty_subst
-                 ++env_ty_subst
-                 ++ty_subst_lang
-                 ++block_parameterized++val_parameterized
-                 ++ty_env_lang)
-              exists_cps_def
-              exists_cps
-              exists_lang)
-  as exists_cps_preserving.
-Proof.
-  (*TODO: takes much longer than legacy auto_elab_compiler (has not terminated). Why?
-    Time  1:Automation.auto_elab_compiler.
-    Legacy: ~50s
-   *)
-  auto_elab_compiler.
-Qed.
-#[local] Definition exists_cps_entry :=
-  cmp_entry (elab_compiler_implies_preserving exists_cps_preserving).
-#[export] Hint Resolve exists_cps_entry : preserving_db.
 
 Definition tgt_parameterized :=
   let ps := (elab_param "D" (tgt_ext ++ block_subst
@@ -840,6 +88,19 @@ Definition cc_parameterized :=
     parameterize_compiler "D"
       ptgt pir cc_full.
 
+(* TODO: duplicated from PolyCompilerLangs. Should the definition be non-local?*)
+Local Definition bvp' :=
+  let ps := (elab_param "D" (ir_ext
+                               ++ block_subst
+                                 ++ value_subst)
+               [("sub", Some 2);
+                ("ty", Some 0);
+                ("env", Some 0);
+                ("val",Some 2);
+                ("blk",Some 1)]) in
+  parameterize_lang "D" {{s #"ty_env"}}
+    ps (block_subst ++ value_subst).
+
 Lemma cc_parameterized_correct
   : preserving_compiler_ext
       (tgt_Model:=core_model ((tgt_parameterized
@@ -883,7 +144,7 @@ Qed.
   cmp_entry cc_parameterized_correct.
 #[export] Hint Resolve cc_parameterized_entry : preserving_db.
 
-Definition exists_cc_def : compiler string :=
+Definition exists_cc_def : compiler :=
   match # from exists_block_lang with
   | {{e #"Exists" "D" "A"}} =>
       {{e #"Exists" "A" }}
@@ -926,7 +187,7 @@ Proof. auto_elab. Qed.
 
 #[local] Definition cmp'' := Eval compute in cc_parameterized.
 
-Definition block_ty_subst_cc_def : compiler string :=
+Definition block_ty_subst_cc_def : compiler :=
   match # from (block_param_substs
                   ++val_param_substs ++ block_ty_subst
                   ++env_ty_subst) with
@@ -984,7 +245,7 @@ Derive exists_cc
               exists_block_lang)
   as exists_cc_preserving.
 Proof.
-  auto_elab_compiler.
+  ElabCompilers.auto_elab_compiler.
   { apply TODO (*Automation.by_reduction; Matches.t'.*). }
   {
     
@@ -1033,7 +294,6 @@ Qed.
   cmp_entry (elab_compiler_implies_preserving exists_cc_preserving).
 #[export] Hint Resolve exists_cc_cmp_entry : preserving_db.
 
-From Pyrosome.Compilers Require Import CompilerTransitivity.
 
   Local Notation preserving_compiler_ext' tgt cmp_pre cmp src :=
     (preserving_compiler_ext (tgt_Model:=core_model tgt) cmp_pre cmp src).
@@ -1112,8 +372,9 @@ Proof.
   Qed.
 
   
-  Definition hide_cmp_implicits (l:lang) : compiler string -> compiler string :=
+  Definition hide_cmp_implicits (l:lang) : compiler -> compiler :=
     NamedList.named_map (hide_ccase_implicits l).
+  
   #[local] Definition id_cps_def :=
         Eval compute in
         hide_cmp_implicits
@@ -1125,6 +386,7 @@ Proof.
                       ++ val_ty_subst
                       ++env_ty_subst
                       ++ty_subst_lang)).
+  
 Lemma ty_subst_lang_id_ext
   : preserving_compiler_ext
       (cps_parameterized ++ ty_env_cmp)
