src/Pyrosome/Lang/PolyCompilerLangs.v
@@ -1,0 +1,367 @@
+From coqutil Require Import Datatypes.String.
+From Stdlib Require Import Lists.List.
+Import ListNotations.
+Open Scope string.
+Open Scope list.
+From Utils Require Import Utils GallinaHintDb.
+From Pyrosome Require Import Theory.Core 
+  Theory.Renaming Compilers.SemanticsPreservingDef
+  Compilers.Compilers Compilers.Parameterizer Compilers.CompilerFacts
+  Elab.Elab Elab.ElabCompilers
+  Tools.CompilerTools Compilers.CompilerTransitivity
+  Tools.Matches Tools.EGraph.Automation
+  Tools.EGraph.TypeInference
+  Tools.EGraph.ComputeWf
+  Tools.Resolution.
+From Pyrosome.Lang Require Import PolySubst
+  SimpleVSubst SimpleVCPS SimpleEvalCtx Let
+  SimpleEvalCtxCPS SimpleUnit NatHeap SimpleVCPSHeap
+  SimpleVFixCPS SimpleVFixCC SimpleVCC SimpleVSTLC
+  SimpleVCCHeap SimpleVFix CombinedThm.
+From Pyrosome.Tools Require Import InjRuleGen.
+Import Core.Notations.
+Import CompilerDefs.Notations.
+
+From Stdlib Require derive.Derive.
+
+Definition stlc_parameterized :=
+    let ps := (elab_param "D" (stlc ++ exp_ret ++ exp_subst_base
+                                 ++ value_subst)
+               [("sub", Some 2);
+                ("ty", Some 0);
+                ("env", Some 0);
+                ("val",Some 2);
+                ("exp",Some 2)]) in
+  parameterize_lang "D" {{s #"ty_env"}}
+    ps stlc.
+
+Local Definition evp' := 
+    let ps := (elab_param "D" (stlc ++exp_ret ++ exp_subst_base
+                                 ++ value_subst)
+               [("sub", Some 2);
+                ("ty", Some 0);
+                ("env", Some 0);
+                ("val",Some 2);
+                ("exp",Some 2)]) in
+  parameterize_lang "D" {{s #"ty_env"}}
+    ps (exp_ret ++ exp_subst_base ++ value_subst).
+
+Lemma stlc_parameterized_wf
+  : wf_lang_ext ((exp_parameterized++val_parameterized)
+                       ++ty_env_lang)
+      stlc_parameterized.
+Proof.
+  change (exp_parameterized++val_parameterized) with evp'.
+  (*TODO: phrase exp_and_val_parameterized as parameterized in definition*)
+  (*TODO: need to strengthen parameterization pl w/ add'l language?
+    Currently cheating.
+   *)
+  eapply parameterize_lang_preserving_ext;
+    try typeclasses eauto;
+    [repeat t';  constructor (*TODO: include in t'*)
+    | now prove_by_lang_db..
+    | vm_compute; exact I].
+Qed.
+#[local] Definition stlc_parameterized_entry :=
+  lang_entry stlc_parameterized_wf.
+#[export] Hint Resolve stlc_parameterized_entry : wf_lang_db.
+
+Definition src_parameterized :=
+    let ps := (elab_param "D" (let_lang ++ src_ext ++ exp_ret ++ exp_subst_base
+                                 ++ value_subst)
+               [("sub", Some 2);
+                ("ty", Some 0);
+                ("env", Some 0);
+                ("val",Some 2);
+                ("exp",Some 2)]) in
+  parameterize_lang "D" {{s #"ty_env"}}
+    ps (let_lang ++ src_ext).
+
+Local Definition evp'' := 
+    let ps := (elab_param "D" (let_lang ++ src_ext ++exp_ret ++ exp_subst_base
+                                 ++ value_subst)
+               [("sub", Some 2);
+                ("ty", Some 0);
+                ("env", Some 0);
+                ("val",Some 2);
+                ("exp",Some 2)]) in
+  parameterize_lang "D" {{s #"ty_env"}}
+    ps (exp_subst ++ value_subst).
+
+(*TODO: move to Core.v*)
+Lemma wf_lang_concat' (l_pre l1 l2 : lang)
+  : wf_lang_ext l_pre l1 ->
+    wf_lang_ext (l1++l_pre) l2 ->
+    wf_lang_ext l_pre (l2 ++ l1).
+Proof.
+  induction 2; basic_goal_prep; basic_core_firstorder_crush.
+  rewrite <- app_assoc; eauto.
+Qed.
+
+Lemma src_parameterized_wf
+  : wf_lang_ext ((exp_parameterized++val_parameterized)
+                       ++ty_env_lang)
+      src_parameterized.
+Proof.
+  change (exp_parameterized++val_parameterized) with evp''.
+  eapply parameterize_lang_preserving_ext;
+    try typeclasses eauto;
+    [repeat t';  constructor (*TODO: include in t'*)
+    | try now prove_by_lang_db..
+    | vm_compute; exact I].
+Qed.
+#[local] Definition src_parameterized_entry :=
+  lang_entry src_parameterized_wf.
+#[export] Hint Resolve src_parameterized_entry : wf_lang_db.
+
+
+
+
+
+Definition ir_parameterized :=
+  let ps := (elab_param "D" (ir_ext ++ block_subst
+                                 ++ value_subst)
+               [("sub", Some 2);
+                ("ty", Some 0);
+                ("env", Some 0);
+                ("val",Some 2);
+                ("blk",Some 1)]) in
+  parameterize_lang "D" {{s #"ty_env"}}
+    ps ir_ext.
+
+Local Definition bvp' :=
+  let ps := (elab_param "D" (ir_ext
+                               ++ block_subst
+                                 ++ value_subst)
+               [("sub", Some 2);
+                ("ty", Some 0);
+                ("env", Some 0);
+                ("val",Some 2);
+                ("blk",Some 1)]) in
+  parameterize_lang "D" {{s #"ty_env"}}
+    ps (block_subst ++ value_subst).
+
+Lemma ir_parameterized_wf
+  : wf_lang_ext ((block_parameterized++
+                       val_parameterized)
+                       ++ty_env_lang)
+      ir_parameterized.
+Proof.
+  change (block_parameterized++val_parameterized) with bvp'.
+  eapply parameterize_lang_preserving_ext;
+    try typeclasses eauto;
+    [repeat t';  constructor (*TODO: include in t'*)
+    | try now  prove_by_lang_db..
+    | vm_compute; exact I].
+Qed.
+#[local] Definition ir_parameterized_entry :=
+  lang_entry ir_parameterized_wf.
+#[export] Hint Resolve ir_parameterized_entry : wf_lang_db.
+
+Definition exists_def : lang :=
+  {[l (*l/subst TODO: psubst*)
+  [:| "D" : #"ty_env", "A" : #"ty" (#"ty_ext" "D")
+      -----------------------------------------------
+      #"Exists" "A" : #"ty" "D"
+  ];
+    (*TODO:autogenerate*)
+  [:= "D" : #"ty_env",
+      "A" : #"ty" (#"ty_ext" "D"),
+      "D'" : #"ty_env",
+      "d" : #"ty_sub" "D'" "D"
+      ----------------------------------------------- ("ty_subst Exists")
+      #"ty_subst" "d" (#"Exists" "A")
+      = #"Exists" (#"ty_subst" (#"ty_snoc" (#"ty_cmp" #"ty_wkn" "d") #"ty_hd") "A")
+      : #"ty" "D'"
+   ];
+    [:| "D" : #"ty_env",
+       "G" : #"env" "D",
+       "A" :  #"ty" "D",
+       "B" :  #"ty" (#"ty_ext" "D"),
+       "v" : #"val" "D" "G" (#"ty_subst" (#"ty_snoc" #"ty_id" "A") "B")
+       -----------------------------------------------
+       #"pack_val" "A" "v" : #"val" "D" "G" (#"Exists" "B")
+  ];
+    [:| "D" : #"ty_env",
+       "G" : #"env" "D",
+       "A" :  #"ty" "D",
+       "B" :  #"ty" (#"ty_ext" "D"),
+       "e" : #"exp" "D" "G" (#"ty_subst" (#"ty_snoc" #"ty_id" "A") "B")
+       -----------------------------------------------
+       #"pack" "A" "e" : #"exp" "D" "G" (#"Exists" "B")
+  ];
+  [:| "D" : #"ty_env",
+      "G" : #"env" "D",
+      "B" : #"ty" (#"ty_ext" "D"),
+      "e" : #"exp" "D" "G" (#"Exists" "B"),
+      "C" : #"ty" "D",
+      "e'" : #"exp" (#"ty_ext" "D") (#"ext" (#"env_ty_subst" #"ty_wkn" "G") "B")
+               (#"ty_subst" #"ty_wkn" "C")
+       -----------------------------------------------
+       #"unpack" "e" "e'" : #"exp" "D" "G" "C"
+  ];
+  [:=  "D" : #"ty_env",
+       "G" : #"env" "D",
+       "A" :  #"ty" "D",
+       "B" :  #"ty" (#"ty_ext" "D"),
+       "v" : #"val" "D" "G" (#"ty_subst" (#"ty_snoc" #"ty_id" "A") "B"),
+      "C" : #"ty" "D",
+      "e'" : #"exp" (#"ty_ext" "D") (#"ext" (#"env_ty_subst" #"ty_wkn" "G") "B")
+               (#"ty_subst" #"ty_wkn" "C")
+      ----------------------------------------------- ("unpack-beta")
+      #"unpack" (#"ret" (#"pack_val" "A" "v")) "e'"
+      = #"exp_subst" (#"snoc" #"id" "v") (#"exp_ty_subst" (#"ty_snoc" #"ty_id" "A") "e'")
+      : #"exp" "D" "G" "C"
+  ]
+  ]}.
+
+#[local] Definition Exists_inst_for_db := inst_for_db "Exists".
+#[export] Hint Resolve Exists_inst_for_db : injective_con.
+
+Definition exists_lang :=
+  Eval vm_compute in
+    (infer_lang_ext_simple_incr 10 100
+       (exp_param_substs
+          ++ exp_ty_subst
+          ++ val_param_substs
+          ++ val_ty_subst
+          ++env_ty_subst
+          ++ty_subst_lang
+          ++exp_parameterized++val_parameterized
+          ++ty_env_lang) exists_def).
+
+
+Lemma exists_lang_wf : wf_lang_ext (exp_param_substs
+                             ++ exp_ty_subst
+                             ++ val_param_substs
+                             ++ val_ty_subst
+                             ++env_ty_subst
+                             ++ty_subst_lang
+                             ++exp_parameterized++val_parameterized
+                             ++ty_env_lang)
+                               exists_lang.
+Proof. compute_wf_lang. Qed.
+#[local] Definition exists_lang_entry :=
+  lang_entry exists_lang_wf.
+#[export] Hint Resolve exists_lang_entry : wf_lang_db.
+
+Definition exists_block_def : lang :=
+  {[l (*l/subst TODO: psubst*)
+  [:| "D" : #"ty_env", "A" : #"ty" (#"ty_ext" "D")
+      -----------------------------------------------
+      #"Exists" "A" : #"ty" "D"
+  ];
+    [:= "D" : #"ty_env",
+              "A" : #"ty" (#"ty_ext" "D"),
+              "D'" : #"ty_env",
+              "d" : #"ty_sub" "D'" "D"
+              ----------------------------------------------- ("ty_subst Exists")
+              #"ty_subst" "d" (#"Exists" "A")
+               = #"Exists" (#"ty_subst" (#"ty_snoc" (#"ty_cmp" #"ty_wkn" "d") #"ty_hd") "A")
+               : #"ty" "D'"
+          ];
+    [:| "D" : #"ty_env",
+       "G" : #"env" "D",
+       "A" :  #"ty" "D",
+       "B" :  #"ty" (#"ty_ext" "D"),
+       "v" : #"val" "D" "G" (#"ty_subst" (#"ty_snoc" #"ty_id" "A") "B")
+       -----------------------------------------------
+       #"pack" "A" "v" : #"val" "D" "G" (#"Exists" "B")
+  ];
+  [:| "D" : #"ty_env",
+      "G" : #"env" "D",
+      "B" : #"ty" (#"ty_ext" "D"),
+      "v" : #"val" "D" "G" (#"Exists" "B"),
+      "e" : #"blk" (#"ty_ext" "D") (#"ext" (#"env_ty_subst" #"ty_wkn" "G") "B")
+       -----------------------------------------------
+       #"unpack" "v" "e" : #"blk" "D" "G"
+  ];
+  [:=  "D" : #"ty_env",
+       "G" : #"env" "D",
+       "A" :  #"ty" "D",
+       "B" :  #"ty" (#"ty_ext" "D"),
+       "v" : #"val" "D" "G" (#"ty_subst" (#"ty_snoc" #"ty_id" "A") "B"),
+      "e" : #"blk" (#"ty_ext" "D") (#"ext" (#"env_ty_subst" #"ty_wkn" "G") "B")
+      ----------------------------------------------- ("unpack-beta")
+      #"unpack" (#"pack" "A" "v") "e"
+      = #"blk_subst" (#"snoc" #"id" "v") (#"blk_ty_subst" (#"ty_snoc" #"ty_id" "A")"e")
+      : #"blk" "D" "G"
+  ];
+  [:= "D" : #"ty_env",
+      "G" : #"env" "D",
+      "B" : #"ty" (#"ty_ext" "D"),
+      "v" : #"val" "D" "G" (#"Exists" "B"),
+      "e" : #"blk" "D" (#"ext" "G" (#"Exists" "B"))
+       ----------------------------------------------- ("unpack-eta")
+       #"unpack" "v" (#"blk_subst" (#"snoc" #"wkn" (#"pack" #"ty_hd" #"hd"))
+                        (#"blk_ty_subst" #"ty_wkn" "e"))
+       = #"blk_subst" (#"snoc" #"id" "v") "e"
+       : #"blk" "D" "G"
+  ];
+   [:= "D" : #"ty_env",
+       "G" : #"env" "D",
+       "A" :  #"ty" "D",
+       "B" :  #"ty" (#"ty_ext" "D"),
+       "v" : #"val" "D" "G" (#"ty_subst" (#"ty_snoc" #"ty_id" "A") "B"),
+      "G'" : #"env" "D",
+      "g" : #"sub" "D" "G'" "G"
+       ----------------------------------------------- ("blk_subst pack")
+       #"val_subst" "g" (#"pack" "A" "v")
+       = #"pack" "A" (#"val_subst" "g" "v")
+       : #"val" "D" "G'" (#"Exists" "B")
+  ];
+  [:= "D" : #"ty_env",
+      "G" : #"env" "D",
+      "B" : #"ty" (#"ty_ext" "D"),
+      "v" : #"val" "D" "G" (#"Exists" "B"),
+      "e" : #"blk" (#"ty_ext" "D") (#"ext" (#"env_ty_subst" #"ty_wkn" "G") "B"),
+      "G'" : #"env" "D",
+      "g" : #"sub" "D" "G'" "G"
+       ----------------------------------------------- ("blk_subst unpack")
+       #"blk_subst" "g" (#"unpack" "v" "e")
+       = #"unpack" (#"val_subst" "g" "v")
+           (#"blk_subst" { under {{e #"sub_ty_subst" #"ty_wkn" "g" }} } "e")
+       : #"blk" "D" "G'"
+  ]
+  ]}.
+
+
+Definition exists_block_lang' :=
+  Eval vm_compute in
+    (infer_lang_ext_simple_incr 10 100
+       (block_param_substs
+          ++val_param_substs
+          ++ block_ty_subst
+          ++env_ty_subst
+          ++ty_subst_lang
+          ++block_parameterized++val_parameterized
+          ++ty_env_lang)
+       exists_block_def).
+
+(*TODO: too slow. Why? should replace the derive below.
+Lemma exists_block_lang_wf
+  : wf_lang_ext (block_param_substs
+                   ++val_param_substs
+                   ++ block_ty_subst
+                   ++env_ty_subst
+                   ++ty_subst_lang
+                   ++block_parameterized++val_parameterized
+                   ++ty_env_lang)
+      exists_block_lang.
+Proof. compute_wf_lang. Qed.
+*)
+
+Derive exists_block_lang
+  in (elab_lang_ext (block_param_substs
+                             ++val_param_substs
+                             ++ block_ty_subst
+                             ++env_ty_subst
+                             ++ty_subst_lang
+                             ++block_parameterized++val_parameterized
+                             ++ty_env_lang)
+              exists_block_def exists_block_lang)
+       as exists_block_lang_wf.
+Proof. auto_elab. Qed.
+#[local] Definition exists_block_lang_entry :=
+  lang_entry (elab_lang_implies_wf exists_block_lang_wf).
+#[export] Hint Resolve exists_block_lang_entry : wf_lang_db.
